\documentclass{beamer}
\usetheme{CambridgeUS}



\usepackage{enumitem}
\usepackage{tfrupee}
\usepackage{amsmath}
\usepackage{amssymb}
\usepackage{gensymb}
\usepackage{graphicx}
\usepackage{txfonts}

\def\inputGnumericTable{}

\usepackage[latin1]{inputenc}                                 
\usepackage{color}                                            
\usepackage{array}                                            
\usepackage{longtable}                                        
\usepackage{calc}                                             
\usepackage{multirow}                                         
\usepackage{hhline}                                           
\usepackage{ifthen}
\usepackage{caption} 
\captionsetup[table]{skip=3pt}  
\providecommand{\pr}[1]{\ensuremath{\Pr\left(#1\right)}}
\providecommand{\cbrak}[1]{\ensuremath{\left\{#1\right\}}}
\renewcommand{\thefigure}{\arabic{table}}
\renewcommand{\thetable}{\arabic{table}}                                     

\title{AI1110 \\ Assignment 11}
\author{MANIKANTA UPPULAPU \\ (BT05)}
\date{\today}


\begin{document}
	\begin{frame}
		\titlepage
	\end{frame}
	\begin{frame}{Outline}
		\tableofcontents
	\end{frame}
	\section{Question}
	\begin{frame}{Problem Statement}
	\begin{block}
{Question:}	 Given a discrete type random variable n taking the values 1,2,\dots and a sequence of random variables $X_k$ independent  of  n, we form the sum \\
$$ S = \sum_{k=1}^{n} x_k$$\\
This sum is a random variable specified as follows: For a specific $\zeta$,n($\zeta$) is an integer and s($\zeta$) equals the sum of the numbers X_k($\zeta$) for k from 1 to n($\zeta$). We maintain that if the random variables $X_k$ have the same mean, then
$$E\{s\}=\eta E\{n\} , \text{where} E\{x_k\} = \eta$$

\end{block}
\end{frame}
	\section{Solution}
	\begin{frame}{Solution}
Clearly,$E\{x_k|n=n\} = E\{X_k\}$ beacuse $x_k$ is independent of $n$.\\
Hence\\
\begin{align}
E\{s|n=n\} = E\cbrak{\sum_{k=1}^{n}x_k|n=n} = \sum_{k=1}^{n}E\{x_k\}=\eta n\label{eq1}
\end{align}
from \eqref{eq1} and $E\{g(x,y)|x\}$ = \int_{-\infty}^{\infty} g(x,y)f(y|x)dy\\
\begin{align}
E\{s\} = E\{E\{s|n\}\} = E \{\eta n\}
\end{align}
\end{frame}

\begin{frame}{Solution}
if the random variables $x_k$ are uncorrelated with the same variance \sigma^2,then\\
\begin{align}
 E\{s^2\} = \eta^2 E\{n^2\} + \sigma^2 E\{n\}\\
 \implies E\{s^2|n=n\} = \sum_{i=1}^{n}\sum_{k=1}^{n}E\{x_ix_k\}\\
 \text{where} E\{x_ix_k\} =\begin{cases}
  \sigma^2 + \eta^2 & i = k \\
 \eta^2 & i \neq k
 \end{cases}
\end{align}
\end{frame}
\begin{frame}{Solution}
    with i = k and $ n^2 - n$ terms with i \neq k \\
     \begin{align}
\implies (\sigma^2+\eta^2)n + \eta^2(n^2-n) = \eta^2 n^2 + \sigma^2 n 
 \end{align}
 this yields because\\
 \begin{align}
  E\{s^2\} = E\{E\{s^2|n\}\} = E\{\eta^2 n^2 + \sigma^2 n\}
  \end{align}
\end{frame}
\end{document}
